Refactor [pow2] example, add comments

doc/tutorial/pow2.v
@@ -3,8 +3,11 @@ From compcert Require Import Coqlib Integers Floats AST Ctypes Cop Clight Clight
 From compcert Require Import Maps Values ClightBigstep Events.
 
 Require Import Clight.pow2.
+
 Open Scope Z_scope.
 
+
+(** aliases for clarity **)
 Definition Vnat (n : nat) := Vint (Int.repr (Z.of_nat n)).
 Definition Mset' := Maps.PTree.set.
 Definition Mset := Mset' val.
@@ -12,25 +15,17 @@ Definition Mset := Mset' val.
 Ltac gso_simpl := rewrite PTree.gso by discriminate.
 Ltac gss_simpl := rewrite PTree.gss.
 
-Lemma succ_not_zero_int (n : nat) :
-  Z.of_nat (S n) < Int.modulus ->
-  Int.repr (Z.of_nat (S n)) <> Int.repr (Z.of_nat O).
-Proof.
-  intros; intro H1.
-  apply f_equal with (f := Int.unsigned) in H1.
-  repeat rewrite Int.unsigned_repr_eq in H1.
-  rewrite Zmod_small, Zmod_0_l in H1
-    by (auto with zarith).
-  inversion H1.
-Qed.
 
+(** functional specification **)
 Definition pow2_fspec (n : nat) := Nat.pow 2 n.
 
-Lemma pow2_fspec_S_geq_2 (n : nat) :
-  (2 <= pow2_fspec (S n))%nat.
+
+(** aux arithmetic lemmas **)
+Lemma pow2_fspec_positive (n : nat) :
+  (1 <= pow2_fspec n)%nat.
 Proof.
   unfold pow2_fspec.
-  assert (2 = 2^1)%nat by trivial; rewrite H at 1; clear H.
+  assert (1 = 2^0)%nat by trivial; rewrite H at 1; clear H.
   apply Nat.pow_le_mono_r; lia.
 Qed.
 
@@ -42,6 +37,59 @@ Proof.
   lia.
 Qed.
 
+Lemma succ_not_zero_int (n : nat) :
+  Z.of_nat (S n) < Int.modulus ->
+  Int.eq (Int.repr (Z.of_nat (S n))) Int.zero = false.
+Proof.
+  intro.
+  apply Int.eq_false.
+  intro H1.
+  unfold Int.zero in H1.
+  apply f_equal with (f := Int.unsigned) in H1.
+  repeat rewrite Int.unsigned_repr_eq in H1.
+  rewrite Zmod_small, Zmod_0_l in H1
+    by (auto with zarith).
+  inversion H1.
+Qed.
+
+Fact int_max_unsigned_lower_bound :
+  4294967295 <= Int.max_unsigned.
+Proof.
+  unfold Int.max_unsigned, Int.modulus, Int.wordsize, Wordsize_32.wordsize.
+  cbn; lia.
+Qed.
+
+Lemma S_sub_1_int (n : nat) :
+  Z.of_nat (S n) < Int.modulus ->
+  Vint (Int.sub (Int.repr (Z.of_nat (S n))) (Int.repr 1)) = Vnat n.
+Proof.
+  intro.
+  unfold Int.sub.
+  repeat rewrite Int.unsigned_repr. replace (Z.of_nat (S n) - 1) with (Z.of_nat n) by lia.
+  reflexivity.
+  pose proof int_max_unsigned_lower_bound; lia.
+  unfold Int.max_unsigned; lia.
+Qed.
+
+Lemma sum_n_n_2n_int (n : nat) :
+  Z.of_nat n < Int.modulus ->
+  Vint (Int.add (Int.repr (Z.of_nat n)) (Int.repr (Z.of_nat n))) = Vnat (n * 2).
+Proof.
+  intro.
+  unfold Int.add.
+  repeat rewrite Int.unsigned_repr.
+  replace (Z.of_nat n + Z.of_nat n) with (Z.of_nat (n * 2)) by lia.
+  reflexivity.
+  unfold Int.max_unsigned.
+  lia.
+Qed.
+
+
+
+(** * correctness proofs *)
+Definition f_pow2_statement := f_pow2.(fn_body).
+
+(* pull out a part of the AST corresponding to the loop *)
 Definition f_pow2_loop :=
   (Swhile
     (Etempvar _n tuint)
@@ -52,126 +100,132 @@ Definition f_pow2_loop :=
         (Ebinop Osub (Etempvar _n tuint) (Econst_int (Int.repr 1) tint)
           tuint)))).
 
-Lemma f_pow2_loop_correct : forall ge e m, forall n res le,
-      Z.of_nat n < Int.modulus ->
-      Z.of_nat res < Int.modulus ->
-      Z.of_nat (res * (pow2_fspec n)) < Int.modulus ->
-      
-      le!_n = Some (Vnat n) ->
-      le!_res = Some (Vnat res) ->
-      
-      exists t le',
-        exec_stmt ge e le m f_pow2_loop t le' m Out_normal
-        /\ (le'!_res) = Some (Vnat (res * (pow2_fspec n))).
+(*
+ * prove corretness of the loop * in isolation from other parts of the function
+ * If "res" is bound to an arbitrary value [res] at the beginning
+ * then the return will be [res] multiplied by [2] [n] times.
+ *
+ * This is a generalization, since "res" is normally initially bound to [1],
+ * but it actually allows for an easier proof, simplifying induction
+ *)
+Lemma f_pow2_loop_correct : forall n ge e ste m res,
+  Z.of_nat n < Int.modulus ->
+  Z.of_nat (res * (pow2_fspec n)) < Int.modulus ->
+  
+  ste ! _n = Some (Vnat n) ->
+  ste ! _res = Some (Vnat res) ->
+  
+  exists t rte,
+    exec_stmt ge e ste m f_pow2_loop t rte m Out_normal /\
+    (rte ! _res) = Some (Vnat (res * (pow2_fspec n))).
 Proof.
   induction n; intros.
-  - repeat eexists.
-    + eapply exec_Sloop_stop1.
-      eapply exec_Sseq_2.
+  - (* iBase *)
+    repeat eexists.
+
+    (* the loop must stop *)
+    eapply exec_Sloop_stop1.
+    (* the sequence terminates on first (left) statement with a break *)
+    eapply exec_Sseq_2.
+
+    repeat econstructor.
+    all: try eassumption.
+    all: try econstructor.
+    discriminate.
+    unfold pow2_fspec; simpl Nat.pow; rewrite Nat.mul_1_r.
+    assumption.
+  - (* iStep *)
+
+    (* this is the [te] after one iteration of the loop - the one to apply induction hypothesis on *)
+    remember (PTree.set _n (Vint (Int.sub (Int.repr (Z.of_nat (S n))) (Int.repr 1)))
+               (PTree.set _res (Vint (Int.add (Int.repr (Z.of_nat res)) (Int.repr (Z.of_nat res))))
+                 ste))
+      as sIte.
+
+    (* prepare induction hypothesis *)
+    pose proof IHn ge e sIte m (res * 2)%nat as IH.
+    destruct IH as [t IH];
+      [ lia
+      | rewrite pow2_fspec_S in H0; lia
+      | subst; gss_simpl; rewrite S_sub_1_int by assumption; reflexivity
+      | subst; gso_simpl; gss_simpl;
+          rewrite sum_n_n_2n_int by (pose proof pow2_fspec_positive (S n); nia);
+          reflexivity
+      |].
+    destruct IH as [rIte IH]; destruct IH as [IH1 IH2].
+    
+    repeat eexists.
+    + (* the loop continues for one iteration *)
+      eapply exec_Sloop_loop.
       repeat econstructor.
-      all: repeat econstructor.
-      all: try eassumption; try discriminate.
+      eassumption.
       econstructor.
-      econstructor.
-    + replace (res * pow2_fspec 0)%nat with res
-        by (rewrite Nat.mul_1_r; reflexivity).
+      rewrite succ_not_zero_int. econstructor.
       assumption.
-  - assert
-      (
-        let step_le := (Mset _n (Vnat n)
-                            (Mset _res (Vnat (res * 2))
-                                  le)) in
-        exists (t : trace) (le' : temp_env),
-          exec_stmt ge e step_le m f_pow2_loop t le' m Out_normal
-          /\
-          le' ! _res =  Some (Vnat ((res * 2) * (pow2_fspec n) ))
-      ).
-    {
-      intro; subst step_le.
-      apply IHn.
-      - lia.
-      - pose proof pow2_fspec_S_geq_2 n.
-        nia.
-      - rewrite <-Nat.mul_assoc, <-pow2_fspec_S.
-        assumption.
-      - apply PTree.gss.
-      - gso_simpl; gss_simpl; reflexivity.
-    }
-    destruct H4. destruct H4. destruct H4.
-    repeat eexists;
-     [| rewrite pow2_fspec_S, Nat.mul_assoc; eassumption].
-    eapply exec_Sloop_loop.
-    eapply exec_Sseq_1.
-    2: eapply exec_Sseq_1.
-    econstructor.
-    econstructor.
-    eassumption.
-    econstructor.
-    rewrite Int.eq_false
-       by (apply succ_not_zero_int; assumption); simpl.
-    econstructor.
-    repeat econstructor.
-    eassumption.
-    eassumption.
-    repeat econstructor.
-    repeat econstructor.
-    gso_simpl; eassumption.
-    repeat econstructor.
-    econstructor.
-    econstructor.
-    replace 
-      (PTree.set _n (Vint (Int.sub (Int.repr (Z.of_nat (S n)))
-                                       (Int.repr 1)))
-        (PTree.set _res (Vint (Int.add (Int.repr (Z.of_nat res))
-                                          (Int.repr (Z.of_nat res))))
-          le))
-      with
-        (Mset _n (Vnat n)
-                  (Mset _res (Vnat (res * 2))
-                        le)).
-    eassumption.
-    unfold Mset, Mset', Vnat.
-    repeat f_equal.
-    1: unfold Int.sub.
-    2: unfold Int.add.
-    all: repeat rewrite Int.unsigned_repr_eq;
-      f_equal; repeat rewrite Zmod_small; nia.
+      eassumption.
+      eassumption.
+      econstructor.
+      gso_simpl; eassumption.
+      econstructor.
+      constructor.
+      econstructor.
+
+      (** induction hypothesis applied here *)
+      (* after some folding *)
+      replace
+        (Sloop
+         (Ssequence (Sifthenelse (Etempvar _n tuint) Sskip Sbreak)
+            (Ssequence (Sset _res (Ebinop Oadd (Etempvar _res tuint) (Etempvar _res tuint) tuint))
+               (Sset _n (Ebinop Osub (Etempvar _n tuint) (Econst_int (Int.repr 1) tint) tuint)))) Sskip)
+        with f_pow2_loop
+        by reflexivity.
+      rewrite <-HeqsIte.
+      eassumption.
+    + rewrite IH2; unfold pow2_fspec.
+      rewrite Nat.pow_succ_r by lia; rewrite Nat.mul_assoc.
+      reflexivity.
 Qed.
 
-Theorem f_pow2_correct : forall ge e m n le,
+(** full correctness statement *)
+Theorem f_pow2_correct : forall n ge e ste m,
     Z.of_nat n < Int.modulus ->
     Z.of_nat (pow2_fspec n) < Int.modulus ->
-    le!_n = Some (Vnat n) ->
-    exists t le' out,
-      exec_stmt ge e le m (fn_body f_pow2) t le' m out
-      /\
-      (le'!_res) = Some (Vnat (pow2_fspec n)).
+
+    ste ! _n = Some (Vnat n) ->
+
+    exists t rte,
+      exec_stmt ge e ste m f_pow2_statement t rte m
+        (Out_return (Some (Vnat (pow2_fspec n), tuint))).
 Proof.
   intros.
-  assert
-    (
-      exists t le',
-        exec_stmt ge e (Mset _res (Vnat 1) le) m f_pow2_loop t le' m Out_normal
-        /\
-        le' ! _res = Some (Vnat (1 * (pow2_fspec n)))
-    ).
-  {
-    eapply f_pow2_loop_correct.
-    + apply H.
-    + split.
-    + nia.
-    + rewrite PTree.gso. apply H1. cbv. congruence.
-    + apply PTree.gss.
-  }
-  destruct H2. destruct H2.  destruct H2.
-  eexists. eexists.
-  exists (Out_return (Some (Vnat (pow2_fspec n), tuint))).
-  split.
-  + eapply exec_Sseq_1.
-    econstructor. econstructor.
-    eapply exec_Sseq_1.
-    apply H2.
-    repeat econstructor; rewrite Nat.mul_1_l in H3; assumption.
-  + rewrite Nat.mul_1_l in H3.
+
+  remember (PTree.set _res (Vint (Int.repr 1)) ste)
+    as lte.
+  pose proof f_pow2_loop_correct n ge e lte m 1 as LH.
+  destruct LH as [t LH];
+    [ assumption
+    | nia
+    | subst; gso_simpl; assumption
+    | subst; gss_simpl; reflexivity
+    |].
+  destruct LH as [rte LH]; destruct LH as [LH1 LH2].
+
+  repeat eexists.
+  (*
+   * deconstruct the program into three statements:
+   * - [res] initialization
+   * - loop
+   * - return
+   *)
+  econstructor. 2: econstructor.
+  - (* [res] init *)
+    repeat econstructor.
+  - (* loop. loop correctness lemma applied here *)
+    fold f_pow2_loop; rewrite <-Heqlte.
+    eassumption.
+  - (* return *)
+    repeat econstructor.
+    rewrite Nat.mul_1_l in LH2.
     assumption.
 Qed.
+
